Hashmap/HashSet/Basic.lean
@@ -1,0 +1,81 @@
+/-
+Copyright (c) 2024 Lean FRO, LLC. All rights reserved.
+Released under Apache 2.0 license as described in the file LICENSE.
+Authors: Markus Himmel
+-/
+import Hashmap.HashMap.Basic
+
+set_option autoImplicit false
+
+universe u v
+
+variable {α : Type u}
+
+namespace MyLean
+
+namespace HashSet
+
+structure Raw (α : Type u) where
+  inner : HashMap.Raw α Unit
+
+namespace Raw
+
+@[inline] def empty (capacity := 8) : Raw α :=
+  ⟨HashMap.Raw.empty capacity⟩
+
+instance : EmptyCollection (Raw α) where
+  emptyCollection := empty
+
+@[inline] def insert' [BEq α] [Hashable α] (m : Raw α) (a : α) : Raw α × Bool :=
+  let ⟨r, replaced⟩ := m.inner.insert' a ()
+  ⟨⟨r⟩, replaced⟩
+
+@[inline] def insert [BEq α] [Hashable α] (m : Raw α) (a : α) : Raw α :=
+  ⟨m.inner.insert a ()⟩
+
+@[inline] def contains [BEq α] [Hashable α] (m : Raw α) (a : α) : Bool :=
+  m.inner.contains a
+
+def WF [BEq α] [Hashable α] : Raw α → Prop :=
+  fun r => r.inner.WF
+
+theorem WF.empty [BEq α] [Hashable α] {c} : (empty c : Raw α).WF :=
+  HashMap.Raw.WF.empty
+
+theorem WF.emptyc [BEq α] [Hashable α] : (∅ : Raw α).WF :=
+  HashMap.Raw.WF.empty
+
+theorem WF.insert' [BEq α] [Hashable α] {m : Raw α} {a : α} (h : m.WF) : (m.insert' a).1.WF :=
+  HashMap.Raw.WF.insert' h
+
+theorem WF.insert [BEq α] [Hashable α] {m : Raw α} {a : α} (h : m.WF) : (m.insert a).WF :=
+  HashMap.Raw.WF.insert h
+
+end Raw
+
+end HashSet
+
+structure HashSet (α : Type u) [BEq α] [Hashable α] where
+  inner : HashMap α Unit
+
+namespace HashSet
+
+@[inline] def empty [BEq α] [Hashable α] (capacity := 8) : HashSet α :=
+  ⟨HashMap.empty capacity⟩
+
+instance [BEq α] [Hashable α] : EmptyCollection (HashSet α) where
+  emptyCollection := empty
+
+@[inline] def insert' [BEq α] [Hashable α] (m : HashSet α) (a : α) : HashSet α × Bool :=
+  let ⟨r, replaced⟩ := m.inner.insert' a ()
+  ⟨⟨r⟩, replaced⟩
+
+@[inline] def insert [BEq α] [Hashable α] (m : HashSet α) (a : α) : HashSet α :=
+  ⟨m.inner.insert a ()⟩
+
+@[inline] def contains [BEq α] [Hashable α] (m : HashSet α) (a : α) : Bool :=
+  m.inner.contains a
+
+end HashSet
+
+end MyLean
