Hashmap/HashSet/Lemmas.lean
@@ -1,0 +1,57 @@
+/-
+Copyright (c) 2024 Lean FRO, LLC. All rights reserved.
+Released under Apache 2.0 license as described in the file LICENSE.
+Authors: Markus Himmel
+-/
+import Hashmap.HashMap.Lemmas
+import Hashmap.HashSet.Basic
+
+set_option autoImplicit false
+
+universe u v
+
+variable {α : Type u} [BEq α] [Hashable α] [EquivBEq α] [LawfulHashable α]
+
+namespace MyLean.HashSet
+
+namespace Raw
+
+variable (m : Raw α) (h : m.WF)
+
+@[simp] theorem inner_emptyc : (∅ : Raw α).inner = ∅ := rfl
+@[simp] theorem inner_empty {c : Nat} : (empty c : Raw α).inner = HashMap.Raw.empty c := rfl
+
+@[simp]
+theorem contains_empty {a : α} {c : Nat} : (empty c : Raw α).contains a = false := by
+  simp [contains]
+
+@[simp]
+theorem contains_emptyc {a : α} : (∅ : Raw α).contains a = false := by
+  simp [contains]
+
+theorem contains_insert {a k : α} : (m.insert a).contains k = ((a == k) || m.contains k) := by
+  simp [contains, insert, HashMap.Raw.contains_insert _ h]
+
+end Raw
+
+section
+
+variable (m : HashSet α)
+
+@[simp] theorem inner_emptyc : (∅ : HashSet α).inner = ∅ := rfl
+@[simp] theorem inner_empty {c : Nat} : (empty c : HashSet α).inner = HashMap.empty c := rfl
+
+@[simp]
+theorem contains_empty {a : α} {c : Nat} : (empty c : HashSet α).contains a = false := by
+  simp [contains]
+
+@[simp]
+theorem contains_emptyc {a : α} : (∅ : Raw α).contains a = false := by
+  simp [contains]
+
+theorem contains_insert {a k : α} : (m.insert a).contains k = ((a == k) || m.contains k) := by
+  simp [contains, insert, HashMap.contains_insert]
+
+end
+
+end MyLean.HashSet
